Code generation with multiple polyhedra: finally works!

ocaml/conversions.ml
@@ -1,0 +1,40 @@
+open BinNums
+open Datatypes
+
+let coqnat_to_int n =
+  let rec iter n r =
+    match n with
+    | O -> r
+    | S n -> iter n (r + 1)
+  in iter n 0
+
+let int_to_coqnat n =
+  assert (n >= 0);
+  let rec iter n r =
+    match n with
+    | 0 -> r
+    | _ -> iter (n - 1) (S r)
+  in iter n O
+
+let rec coqpos_to_int n =
+  match n with
+  | Coq_xH -> 1
+  | Coq_xO n -> 2 * coqpos_to_int n
+  | Coq_xI n -> 2 * coqpos_to_int n + 1
+
+let rec int_to_coqpos n =
+  assert (n > 0);
+  if n = 1 then Coq_xH
+  else if n land 1 = 0 then Coq_xO (int_to_coqpos (n lsr 1))
+  else Coq_xI (int_to_coqpos (n lsr 1))
+
+let coqZ_to_int n =
+  match n with
+  | Z0 -> 0
+  | Zpos n -> coqpos_to_int n
+  | Zneg n -> - coqpos_to_int n
+
+let int_to_coqZ n =
+  if n = 0 then Z0
+  else if n > 0 then Zpos (int_to_coqpos n)
+  else Zneg (int_to_coqpos (-n))
